pulse/src/checker/Pulse.Checker.Prover.Normalize.fst
@@ -48,7 +48,7 @@ let __normalize_slprop
 
   let v' = PCP.norm_well_typed_term (elab_env g) steps v in
   let v' = Pulse.Simplify.simplify v' in (* NOTE: the simplify stage is unverified *)
-  let v_equiv_v' = VE_Ext _ _ _ (RU.magic ()) in
+  let v_equiv_v' : slprop_equiv g v v' = () in
   (| v', v_equiv_v' |)
 
 let normalize_slprop
@@ -60,9 +60,9 @@ let normalize_slprop
   if use_rewrites_to then
     let rwr = Pulse.Checker.Prover.RewritesTo.get_subst_from_env g in
     let v' = PS.ss_term v rwr in
-    let eq_v_v' : slprop_equiv g v v' = VE_Ext _ _ _ (RU.magic ()) in
+    let eq_v_v' : slprop_equiv g v v' = () in
     let (| v'', eq_v'_v'' |) = __normalize_slprop g v' in
-    (| v'', VE_Trans _ _ _ _ eq_v_v' eq_v'_v'' |)
+    (| v'', () |)
   else
     __normalize_slprop g v
 
