pulse/src/checker/Pulse.Checker.Rewrite.fst
@@ -39,7 +39,7 @@ let check_slprop_equiv_ext r (g:env) (p q:slprop)
       pp q;
     ]
   | Some token ->
-    VE_Ext g p q (RT.Rel_eq_token _ _ _ ())
+    () : slprop_equiv g p q
 
 let check_slprop_equiv_tac r (g:env) (p q:slprop) (tac_tm : term)
 : T.Tac (slprop_equiv g p q)
@@ -75,15 +75,12 @@ let check_slprop_equiv_tac r (g:env) (p q:slprop) (tac_tm : term)
       text "Using tactic:" ^/^ pp tac_tm
     ]
   | Some token ->
-    // Need a VE_ rule to turn an arbitrary proof into a slprop_equiv.
-    // Or use enough core lemmas to show that slprop_equiv implies equality here,
-    // and then use VE_Ext.
-    VE_Ext g p q (RU.magic ())
+    () : slprop_equiv g p q
 
 let rec check_slprop_equiv r (g:env) (p q:slprop)
 : T.Tac (slprop_equiv g p q)
 = if eq_tm p q
-  then VE_Refl g p
+  then ()
   else (
     match inspect_term p, inspect_term q with
     | Tm_ForallSL u1 b1 t1, Tm_ForallSL u2 b2 t2 ->
@@ -96,13 +93,13 @@ let rec check_slprop_equiv r (g:env) (p q:slprop)
         let g' = push_binding g x b1.binder_ppname b1.binder_ty in
         let nx = b1.binder_ppname, x in
         let ext = check_slprop_equiv r g' (open_term_nv t1 nx) (open_term_nv t2 nx) in
-        VE_Fa g x u1 b1 t1 t2 ext
+        ()
       )
       else check_slprop_equiv_ext r g p q
     | Tm_Star p1 p2, Tm_Star q1 q2 ->
       let ext1 = check_slprop_equiv r g p1 q1 in
       let ext2 = check_slprop_equiv r g p2 q2 in
-      VE_Ctxt g p1 p2 q1 q2 ext1 ext2
+      ()
     | _ -> 
       check_slprop_equiv_ext r g p q
   )
@@ -140,6 +137,6 @@ let check
                  (T.moduleof (fstar_env g))
                  "Pulse.Checker.Rewrite.check_slprop_equiv_tac"
   in
-	let d = T_Rewrite _ p q equiv_p_q in
+	let d : st_typing g _ _ = () in
   let (| c,d |) = match_comp_res_with_post_hint d post_hint in
 	prove_post_hint (try_frame_pre false pre_typing (| _,c,d |) res_ppname) post_hint t.range
